
\documentclass{ctexart}
\usepackage{amsmath}


%%%%%%%%%%%%%%%%%%%%%%%%%%%%%%%%%%%%%%%%%%%%%%%%%%%%%%%%%%%%%%%%%%%%%%%%%%%%%%%%%%%%%%%%%%%%%%%%%%%%%%%%%%%%%%%%%%%%%%%%%%%%%%%%%%%%%%%%%%%%%%%%%%%%%%%%%%%%%%%%%%%%%%%%%%%%%%%%%%%%%%%%%%%%%%%%%%%%%%%%%%%%%%%%%%%%%%%%%%%%%%%%%%%%
%TCIDATA{OutputFilter=LATEX.DLL}
%TCIDATA{Version=5.00.0.2552}
%TCIDATA{<META NAME="SaveForMode" CONTENT="1">}
%TCIDATA{Created=Saturday, September 26, 2015 18:16:14}
%TCIDATA{LastRevised=Sunday, September 27, 2015 00:31:22}
%TCIDATA{<META NAME="GraphicsSave" CONTENT="32">}
%TCIDATA{<META NAME="DocumentShell" CONTENT="Scientific Notebook\Blank Document">}
%TCIDATA{CSTFile=Math with theorems suppressed.cst}
%TCIDATA{PageSetup=72,72,72,72,0}
%TCIDATA{AllPages=
%F=36,\PARA{038<p type="texpara" tag="Body Text" >\hfill \thepage}
%}


\newtheorem{theorem}{Theorem}
\newtheorem{acknowledgement}[theorem]{Acknowledgement}
\newtheorem{algorithm}[theorem]{Algorithm}
\newtheorem{axiom}[theorem]{Axiom}
\newtheorem{case}[theorem]{Case}
\newtheorem{claim}[theorem]{Claim}
\newtheorem{conclusion}[theorem]{Conclusion}
\newtheorem{condition}[theorem]{Condition}
\newtheorem{conjecture}[theorem]{Conjecture}
\newtheorem{corollary}[theorem]{Corollary}
\newtheorem{criterion}[theorem]{Criterion}
\newtheorem{definition}[theorem]{Definition}
\newtheorem{example}[theorem]{Example}
\newtheorem{exercise}[theorem]{Exercise}
\newtheorem{lemma}[theorem]{Lemma}
\newtheorem{notation}[theorem]{Notation}
\newtheorem{problem}[theorem]{Problem}
\newtheorem{proposition}[theorem]{Proposition}
\newtheorem{remark}[theorem]{Remark}
\newtheorem{solution}[theorem]{Solution}
\newtheorem{summary}[theorem]{Summary}
\newenvironment{proof}[1][Proof]{\noindent\textbf{#1.} }{\ \rule{0.5em}{0.5em}}


\begin{document}



$a_{kl}$

\bigskip 

$\overset{\infty }{\underset{l=1}{\sum }}a_{kl}=\left( -1\right) ^{k}k%
\overset{\infty }{\underset{l=1}{\sum }}\left( -1\right) ^{l}\left( \frac{1}{%
l+k}-\frac{k}{\left( l+k\right) ^{2}}\right) ,\qquad \left( 1\right) \qquad $%
Let $t=l+k;$

$\overset{\infty }{\underset{l=1}{\sum }}\left( -1\right) ^{l}\left( \frac{1%
}{l+k}-\frac{k}{\left( l+k\right) ^{2}}\right) =\overset{\infty }{\underset{%
t=k+1}{\sum }}\left( -1\right) ^{t-k}\left( \frac{1}{t}-\frac{k}{t^{2}}%
\right) $

=$\overset{\infty }{\underset{t=1}{\sum }}\left( -1\right) ^{t-k}\left( 
\frac{1}{t}-\frac{k}{t^{2}}\right) -\overset{k}{\underset{t=1}{\sum }}\left(
-1\right) ^{t-k}\left( \frac{1}{t}-\frac{k}{t^{2}}\right) \qquad \left(
2\right) $

$\overset{\infty }{\underset{t=1}{\sum }}\left( -1\right) ^{t-k}\left( \frac{%
1}{t}-\frac{k}{t^{2}}\right) =\left( -1\right) ^{k}\overset{\infty }{%
\underset{t=1}{\sum }}\left( -1\right) ^{t}\left( \frac{1}{t}-\frac{k}{t^{2}}%
\right) =\left( -1\right) ^{k}\left( -\ln 2+\frac{k\pi }{12}\right) \qquad
\left( 3\right) $

Substituting $\left( 3\right) $ into $\left( 2\right) $ $\rightarrow \overset%
{\infty }{\underset{l=1}{\sum }}\left( -1\right) ^{l}\left( \frac{1}{l+k}-%
\frac{k}{\left( l+k\right) ^{2}}\right) =\left( -1\right) ^{k}\left( -\ln 2+%
\frac{k\pi }{12}\right) -\overset{k}{\underset{t=1}{\sum }}\left( -1\right)
^{t-k}\left( \frac{1}{t}-\frac{k}{t^{2}}\right) \qquad \left( 4\right) $

Substituting $\left( 4\right) $ into $\left( 1\right) \rightarrow \overset{%
\infty }{\underset{l=1}{\sum }}a_{kl}=k\left( -\ln 2+\frac{k\pi }{12}\right)
-\overset{k}{\underset{t=1}{\sum }}\left( -1\right) ^{t}\left( \frac{k}{t}-%
\frac{k^{2}}{t^{2}}\right) $

$\overset{\infty }{\underset{k=1}{\sum }}\overset{\infty }{\underset{l=1}{%
\sum }}a_{kl}=\underset{n->\infty }{\lim }\overset{n}{\underset{k=1}{\sum }}%
\overset{\infty }{\underset{l=1}{\sum }}a_{kl}=\overset{n}{\underset{k=1}{%
\sum }}\left[ k\left( -\ln 2+\frac{k\pi }{12}\right) -\overset{k}{\underset{%
t=1}{\sum }}\left( -1\right) ^{t}\left( \frac{k}{t}-\frac{k^{2}}{t^{2}}%
\right) \right] $

=$\left( -\ln 2\right) \overset{n}{\underset{k=1}{\sum }}k+\frac{\pi }{12}%
\overset{n}{\underset{k=1}{\sum }}k^{2}-\overset{n}{\underset{k=1}{\sum }}%
\overset{k}{\underset{t=1}{\sum }}\left( -1\right) ^{t}\left( \frac{k}{t}-%
\frac{k^{2}}{t^{2}}\right) $

$\overset{n}{\underset{k=1}{\sum }}\overset{k}{\underset{t=1}{\sum }}\left(
-1\right) ^{t}\left( \frac{k}{t}-\frac{k^{2}}{t^{2}}\right) =\overset{n}{%
\underset{t=1}{\sum }}\overset{n}{\underset{k=t}{\sum }}\left( -1\right)
^{t}\left( \frac{k}{t}-\frac{k^{2}}{t^{2}}\right) $

$=\overset{n}{\underset{t=1}{\sum }}\left( -1\right) ^{t}\left[ \overset{n}{%
\underset{k=1}{\sum }}\left( \frac{k}{t}-\frac{k^{2}}{t^{2}}\right) -%
\underset{k=1}{\overset{t}{\sum }}\left( \frac{k}{t}-\frac{k^{2}}{t^{2}}%
\right) \right] $

$=\overset{n}{\underset{t=1}{\sum }}\left( -1\right) ^{t}\left[ \left( \frac{%
n\left( n+1\right) }{2t}-\frac{n\left( n+1\right) \left( 2n+1\right) }{6t^{2}%
}\right) -\left( \frac{t\left( t+1\right) }{2t}-\frac{t\left( t+1\right)
\left( 2t+1\right) }{6t^{2}}\right) \right] $


\end{document}
